ThoR/Alloy/Syntax/Predicate/PredDecl/predDecl.lean
@@ -6,10 +6,8 @@ Authors: s. file CONTRIBUTORS
 import ThoR.Basic
 
 import ThoR.Alloy.Syntax.Predicate.PredArg.predArg
-import ThoR.Alloy.Syntax.Predicate.PredArg.predArgService
 
 import ThoR.Shared.Syntax.Formula.formula
-import ThoR.Shared.Syntax.Formula.formulaService
 
 import ThoR.Alloy.Syntax.SeparatedNamespace.extendedIdent
 
@@ -65,97 +63,6 @@ namespace Alloy
     -/
     def addPredArg (pd : predDecl) (pa : predArg) : predDecl :=
       {pd with args := pd.args.append [pa]}
-
-    /--
-    Creates a predicate declaration with arguments
-    -/
-    def createWithArgs
-      (name : Name)
-      (args : Syntax.TSepArray `predArg ",")
-      (forms : TSyntaxArray `formula)
-      : predDecl := Id.run do
-
-      let args : List (predArg) :=
-        (args.getElems.map fun (arg) => (predArg.toType arg)).toList
-
-      let forms : List (formula) :=
-        (forms.map fun (f) => (formula.toType f)).toList
-
-      {
-        name := name.toString
-        args := args
-        forms := forms
-      }
-
-    /--
-    Creates a predicate declaration without arguments
-    -/
-    def createWithoutArgs
-      (name : Name)
-      (forms : TSyntaxArray `formula)
-      : predDecl := Id.run do
-
-      let forms : List (formula) :=
-        (forms.map fun (f) => (formula.toType f)).toList
-
-      {
-        name := name.toString
-        args := []
-        forms := forms
-      }
-
-    /--
-    Parses te given syntax to a structure of predDecl if possible
-    -/
-    def toType (pd : TSyntax `predDecl) : predDecl :=
-      match pd with
-        -- pred declaration with args
-        | `(predDecl| pred $name:extendedIdent ($args:predArg,*) {
-            $forms:formula*
-          }) =>
-            predDecl.createWithArgs (extendedIdent.toName name) args forms
-
-        | `(predDecl| pred $name:extendedIdent [$args:predArg,*] {
-            $forms:formula*
-          }) =>
-            predDecl.createWithArgs (extendedIdent.toName name) args forms
-
-        -- pred declaration without args
-        | `(predDecl| pred $name:extendedIdent {
-            $forms:formula*
-          }) =>
-            predDecl.createWithoutArgs (extendedIdent.toName name) forms
-
-        | _ => {name := "PANIC!", args := [], forms := []}
-
-    /--
-    Gets the required definitions for the predicate declaration to work
-    -/
-    def getReqDefinitions
-      (pd : predDecl)
-      : List (String) := Id.run do
-        let mut result : List (String) := []
-
-        for form in pd.forms do
-          result := result ++ form.getReqDefinitions
-
-        return result
-
-    /--
-    Gets the required variables for the predicate declaration to work
-    -/
-    def getReqVariables
-      (pd : predDecl)
-      : List (String) := Id.run do
-        let mut result : List (String) := []
-
-        for arg in pd.args do
-          result := result ++ arg.expression.getReqVariables
-
-        for form in pd.forms do
-          result := result ++ form.getReqVariables
-
-        return result
 
   end predDecl
 
